$V$ - в.п. над $K$. $\varphi \in \text{End}V,\ f,g \in K[x]$. $\gcd(f,g)=1$.
***Теорема***. $\ker(fg)(\varphi)=\ker f(\varphi)\oplus\ker g(\varphi)$.
>[!tldr] D:
>По свойсту НОД:
>$\exists r,s \in K[x]: fr + gs = 1$
>$f(\varphi)r(\varphi)+g(\varphi)s(\varphi)=id_V$
>Посмотрим на $v \in \ker f \cap \ker g$, убедимся что $\ker f \oplus \ker g$.
>$v = id(v)=\underbrace{f(\varphi)(v)}_{=0}\cdot r(\varphi)(v) + \underbrace{g(\varphi)(v)}_{=0}s(\varphi)(v) = 0$
>Теперь пусть $v \in \ker(fg)(\varphi)$.
>$v = \underbrace{f(\varphi)(v)r(\varphi)(v)}_{v_1} + \underbrace{g(\varphi)(v)s(\varphi)(v)}_{v_2}$
>$f(\varphi)(v_2)=s(\varphi)\big((fg)(\varphi)(v)\big)=0\implies v_2 \in \ker f$.
>$g(\varphi)(v_1)=r(\varphi)\big((fg)(\varphi)(v)\big)=0 \implies v_1 \in \ker g$.
>$\implies \ker f(\varphi) \oplus \ker g(\varphi) = \ker(fg)(\varphi)$

***Следствие***. $g =g_1g_2\dotsc g_k,\ g_i \in K[\varphi]$, $g_i$ попарно взаимно простые. Тогда $$\ker g(\varphi)=\bigoplus^k_{i=1}\ker g_i(\varphi)$$
>[!tldr] D:
>индукция по $k$, 1 очев, 2 следствие из теоремы. ну и так далее

---
[[8. Примарное разложение]]